task 1

hw3.thy
@@ -1,4 +1,71 @@
 theory hw3
   imports Main
 begin
+(*1*)
+datatype exp = Var | Const int | Add exp exp | Mult exp exp
+
+fun eval :: "exp ⇒ int ⇒ int" where
+  "eval Var v = v" |
+  "eval (Const e) v = e" |
+  "eval (Add e f) v = (eval e v) + (eval f v)" |
+  "eval (Mult e f) v = (eval e v) * (eval f v)"
+
+value "eval (Var) 6"
+
+fun evalp :: "int list ⇒ int ⇒ int" where
+  "evalp Nil v = 0" |
+  "evalp (Cons x xs) v = x + v * (evalp xs v)"
+
+value "evalp [4, 2, -1, 3] 4"
+fun add_coeff :: "int list ⇒ int list ⇒ int list" where
+  "add_coeff Nil Nil = Nil" |
+  "add_coeff Nil ys = ys" |
+  "add_coeff xs Nil = xs" |
+  "add_coeff (x#xs) (y#ys) = (x+y)#(add_coeff xs ys)"
+
+value "add_coeff [4, 2, -1, 3] [2,3]"
+
+lemma evalp_add[simp] : "evalp (add_coeff xs ys) x = (evalp xs x) + (evalp ys x)"
+  apply(induction xs rule: add_coeff.induct)
+     apply(auto simp add: algebra_simps)
+  done
+
+fun mult :: "int ⇒ int list ⇒ int list" where
+  "mult n Nil = Nil" |
+  "mult n (x#xs) = (n*x)#(mult n xs)"
+
+lemma evalp_mul[simp] : "evalp (mult n xs) v = n * (evalp xs v)"
+  apply(induction xs)
+   apply(auto simp add:algebra_simps)
+  done
+
+fun mult_coeff :: "int list ⇒ int list ⇒ int list" where
+  "mult_coeff Nil ys = Nil" |
+  "mult_coeff (x#xs) ys = add_coeff (mult x ys) (0#(mult_coeff xs ys))"
+
+lemma evalp_mult[simp] : "evalp (mult_coeff xs ys) x = (evalp xs x) * (evalp ys x)"
+  apply(induction xs)
+   apply(auto simp add: algebra_simps)
+  done
+
+fun coeff :: "exp ⇒ int list" where
+"coeff Var = [0,1]" |
+"coeff (Const i) = [i]" |
+"coeff (Add e f) = add_coeff (coeff e) (coeff f)" |
+"coeff (Mult e f) = mult_coeff (coeff e) (coeff f)"
+
+value "coeff (Add (Mult (Const 2) Var) (Mult (Const (-1)) (Mult Var Var)))"
+
+theorem preservation : "evalp (coeff e) x = eval e x"
+  apply(induction e arbitrary: x)
+  using [[simp_trace]]
+     apply(auto)
+  done
+
+(*2*)
+
+(*3*)
+          
+(*4*)
+
 end
